make F⊗⊕ω environment domain props list-based

TabularTypeInterpreter/F⊗⊕ω.lean
@@ -301,6 +301,16 @@ def TypeVar_subst (Δ : Environment) (a : TypeVarId) (A : «Type») := match Δ 
   | typeExt Δ' a' K => Δ'.TypeVar_subst a A |>.typeExt a' K
   | termExt Δ' x A' => Δ'.TypeVar_subst a A |>.termExt x <| A'.TypeVar_subst a A
 
+def typeVarDom : Environment → List TypeVarId
+  | .empty => []
+  | .typeExt Γ a _ => a :: Γ.typeVarDom
+  | .termExt Γ .. => Γ.typeVarDom
+
+def termVarDom : Environment → List TermVarId
+  | .empty => []
+  | .typeExt Γ .. => Γ.termVarDom
+  | .termExt Γ x _ => x :: Γ.termVarDom
+
 end Environment
 
 judgement_syntax a " ≠ " a' : TypeVarNe (id a, a')
@@ -545,45 +555,21 @@ theorem prod_sum : [[Δ ⊢ ⊗ A ≢ ⊕ B]] := fun equ => by
 
 end TypeInequivalence
 
-judgement_syntax a " ∈ " "dom" "(" Δ ")" : TypeVarInEnvironmentDomain (id a)
+judgement_syntax a " ∈ " "dom" "(" Δ ")" : Environment.InTypeVarInDom (id a)
 
-judgement TypeVarInEnvironmentDomain :=
+def Environment.InTypeVarInDom a (Δ : Environment) := a ∈ Δ.typeVarDom
 
-───────────────── head
-a ∈ dom(Δ, a : K)
+judgement_syntax a " ∉ " "dom" "(" Δ ")" : Environment.NotInTypeVarInDom (id a)
 
-a ∈ dom(Δ)
-a ≠ a'
-────────────────── typeVarExt
-a ∈ dom(Δ, a' : K)
+def Environment.NotInTypeVarInDom a Δ := ¬[[a ∈ dom(Δ)]]
 
-a ∈ dom(Δ)
-───────────────── termVarExt
-a ∈ dom(Δ, x : A)
+judgement_syntax x " ∈ " "dom" "(" Δ ")" : Environment.InTermVarInDom (id x)
 
-judgement_syntax a " ∉ " "dom" "(" Δ ")" : TypeVarNotInEnvironmentDomain (id a)
+def Environment.InTermVarInDom x (Δ : Environment) := x ∈ Δ.termVarDom
 
-def TypeVarNotInEnvironmentDomain a Δ := ¬[[a ∈ dom(Δ)]]
+judgement_syntax x " ∉ " "dom" "(" Δ ")" : Environment.NotInTermVarInDom (id x)
 
-judgement_syntax x " ∈ " "dom" "(" Δ ")" : TermVarInEnvironmentDomain (id x)
-
-judgement TermVarInEnvironmentDomain :=
-
-───────────────── head
-x ∈ dom(Δ, x : A)
-
-x ∈ dom(Δ)
-───────────────── typeVarExt
-x ∈ dom(Δ, a : K)
-
-x ∈ dom(Δ)
-x ≠ x'
-────────────────── termVarExt
-x ∈ dom(Δ, x' : A)
-
-judgement_syntax x " ∉ " "dom" "(" Δ ")" : TermVarNotInEnvironmentDomain (id x)
-
-def TermVarNotInEnvironmentDomain x Δ := ¬[[x ∈ dom(Δ)]]
+def Environment.NotInTermVarInDom x Δ := ¬[[x ∈ dom(Δ)]]
 
 judgement_syntax "⊢ " Δ : EnvironmentWellFormedness
 
